Most of put_ok proof - a put is an append on the (key, value) list abstraction

src/KV.v
@@ -25,6 +25,9 @@ Definition empty_valuset : valuset := ($0, @nil valu).
 Definition entry : Type := (addr * valu).
 Definition empty_entry : entry := ($0, $0).
 
+Definition kBase : addr := $0.
+Definition vBase : addr := $1.
+
 Definition list_prefix A (p l : list A) :=
   firstn (length p) l = p.
 
@@ -39,26 +42,16 @@ Qed.
 
 (* Abstract representation of list of (key, value) puts. *)
 Definition rep l (kv_p : kv_pointer) := (exists diskl,
-  array $0 (map (fun e => addr2valu (fst e)) diskl) $2 *
-  array $1 (map snd diskl) $2 *
-  [[ length diskl = wordToNat maxlen / 2 ]] *
+  array kBase (map (fun e => addr2valu (fst e)) diskl) $2 *
+  array vBase (map snd diskl) $2 *
   [[ length l = wordToNat kv_p ]] *
+  [[ length diskl = wordToNat maxlen ]] *
   [[ list_prefix l diskl ]])%pred.
 
 
 (* Key k isn't in the current store. *)
 Definition no_such_put (l : list entry) (k : addr) : Prop :=
   ~ exists v, In (k, v) l.
-
-(*
-Fixpoint is_last_put (l : list entry) (k : addr) (v : valu) :=
-  match l with
-  | nil => False
-  | (k', v') :: tl =>
-    (k = k' /\ v = v' /\ no_such_put l k) \/
-    (is_last_put tl k v)
-  end.
-*)
 
 (* Key k has value v in the current store. *)
 (* Q: Changed from Fixpoint so that I could assert that is_last_put is true
@@ -67,99 +60,125 @@ Inductive is_last_put : (list entry) -> addr -> valu -> Prop :=
   | KV_no_put : forall k,
     is_last_put nil k empty_value
   | KV_key_eq : forall k v tl,
-    no_such_put tl k -> is_last_put ((k, v) :: tl) k v
+    is_last_put (tl ++ [(k, v)]) k v
   | KV_key_neq : forall k v k' v' tl,
-    ~(k = k') \/ v = v' -> is_last_put tl k v -> is_last_put ((k', v') :: tl) k v.
+    k <> k' -> is_last_put tl k v -> is_last_put (tl ++ [(k', v')]) k v.
 
 
 (* Return `value` for the last instance of `key`. *)
-Definition get T (kv_p : kv_pointer) (key : addr) xp cs rx : prog T :=
-  mscs <- MEMLOG.begin xp cs;
-  let2 (mscs, final_value) <- For i < kv_p
-    Ghost F
-    Loopvar current_value <- (mscs, empty_value)
+Definition get T (kv_p : kv_pointer) (key : addr) xp mscs rx : prog T :=
+  mscs <- MEMLOG.begin xp mscs;
+  let^ (mscs, final_value) <- For i < kv_p
+    Ghost [ F l mbase m ]
+    Loopvar [ mscs current_value ]
     Continuation lrx
     Invariant
-      F
+      MEMLOG.rep xp F (ActiveTxn mbase m) mscs *
+      [[ rep l kv_p (list2mem m) ]] *
+      [[ is_last_put (firstn #i l) key current_value ]]
     OnCrash
-      F
+      MEMLOG.rep xp F (ActiveTxn mbase m) mscs
     Begin
-      let2 (mscs, memory_key) <- MEMLOG.read xp i mscs;
-      if (weq memory_key (addr2valu key)) then
-        let2 (mscs, memory_value) <- MEMLOG.read xp (i ^+ $1) mscs;
-        lrx (mscs, memory_value)
-      else
-        lrx current_value
-  Rof;
-  let2 (mscs, ok) <- MEMLOG.commit xp mscs;
-  If (bool_dec ok true) {
-    rx (mscs, final_value)
-  } else {
-    rx (mscs, empty_value)
-  }.
-
-Hint Rewrite map_length.
+      let^ (mscs, memory_key) <- MEMLOG.read_array xp $0 i $2 mscs;
+      If (weq memory_key (addr2valu key)) {
+        let^ (mscs, memory_value) <- MEMLOG.read_array xp $1 i $2 mscs;
+        lrx ^(mscs, memory_value)
+      } else {
+        lrx ^(mscs, current_value)
+      }
+  Rof ^(mscs, empty_value);
+  let^ (mscs, ok) <- MEMLOG.commit xp mscs;
+  rx ^(mscs, final_value).
 
 
-Theorem get_ok: forall kv_p key xp cs,
-  {< mbase F l value,
-  PRE                   MEMLOG.rep xp (NoTransaction mbase) (ms_empty, cs) *
-                        [[ is_last_put l key value ]] *
-                        [[ (rep l kv_p * F)%pred (list2mem mbase) ]]
+Theorem get_ok: forall kv_p key xp mscs,
+  {< mbase MF l,
+  PRE                   MEMLOG.rep xp MF (NoTransaction mbase) mscs *
+                        [[ (rep l kv_p)%pred (list2mem mbase) ]]
 
-  POST:(mscs', rvalue)  MEMLOG.rep xp (NoTransaction mbase) mscs' *
-                        [[ value = rvalue ]] *
-                        [[ is_last_put l key value ]] *
-                        [[ (rep l kv_p * F)%pred (list2mem mbase) ]]
+  POST RET:^(mscs', rvalue)
+                        MEMLOG.rep xp MF (NoTransaction mbase) mscs' *
+                        [[ is_last_put l key rvalue ]]
 
-  CRASH                 MEMLOG.would_recover_old xp mbase \/
-                        (exists m', MEMLOG.might_recover_cur xp mbase m' *
-                        [[ (rep l kv_p * F)%pred (list2mem m') ]])
-  >} get kv_p key xp cs.
+  CRASH                 MEMLOG.would_recover_old xp MF mbase
+  >} get kv_p key xp mscs.
 Proof.
   unfold get. unfold rep.
+  step.
+  step.
+  constructor.
+
+
 Admitted.
 
-Definition put T (kv_p : kv_pointer) (key : addr) (value : valu) xp cs rx : prog T :=
-  mscs <- MEMLOG.begin xp cs;
-  If (weq kv_p maxlen) {
-    let2 (mscs, ok) <- MEMLOG.commit xp mscs;
-    rx (mscs, false)
-  } else {
-    mscs <- MEMLOG.write xp kv_p (addr2valu key) mscs;
-    mscs <- MEMLOG.write xp (kv_p ^+ $1) value mscs;
-    let2 (mscs, ok) <- MEMLOG.commit xp mscs;
+Definition put T (kv_p : kv_pointer) (key : addr) (value : valu) xp mscs rx : prog T :=
+  mscs <- MEMLOG.begin xp mscs;
+    mscs <- MEMLOG.write_array xp $0 kv_p $2 (addr2valu key) mscs;
+    mscs <- MEMLOG.write_array xp $1 kv_p $2 value mscs;
+    let^ (mscs, ok) <- MEMLOG.commit xp mscs;
     If (bool_dec ok true) {
-      rx (mscs, ok)
+      rx ^(mscs, ok)
     } else {
-      rx (mscs, false)
-    }
-  }.
+      rx ^(mscs, false)
+    }.
 
-Theorem put_ok: forall kv_p key value xp cs,
-  {< mbase F l old_value,
-  PRE               MEMLOG.rep xp (NoTransaction mbase) (ms_empty, cs) *
-                    [[ is_last_put l key old_value ]] *
-                    [[ (rep l kv_p * F)%pred (list2mem mbase) ]]
+Theorem put_ok: forall kv_p key value xp mscs,
+  {< mbase F l,
+  PRE               MEMLOG.rep xp F (NoTransaction mbase) mscs *
+                    [[ (rep l kv_p)%pred (list2mem mbase) ]] *
+                    [[ (kv_p < maxlen)%word ]]
 
   (* Q: Does separation logic account for all the is_last_put and rep stuff, or is that necessary here? *)
-  POST:(mscs', ok)  ([[ ok = true /\ is_last_put ((key, value) :: l) key value ]] *
-                     exists m', MEMLOG.rep xp (NoTransaction m') mscs' *
-                     [[ (rep ((key, value) :: l) (kv_p ^+ $2) * F)%pred (list2mem m') ]]) \/
-                    ([[ ok = false /\ is_last_put l key old_value ]] *
-                     ((MEMLOG.rep xp (NoTransaction mbase) mscs' *
-                       [[ (rep l kv_p * F)%pred (list2mem mbase) ]]) \/
-                      (exists m', MEMLOG.rep xp (NoTransaction m') mscs' *
-                       [[ (rep l kv_p * F)%pred (list2mem m') ]])
-                     )
-                    )
+  POST RET:^(mscs', ok)  ([[ ok = true ]] *
+                     exists m', MEMLOG.rep xp F (NoTransaction m') mscs' *
+                     [[ (rep (l ++ [(key, value)]) (kv_p ^+ $1))%pred (list2mem m') ]]) \/
+                    ([[ ok = false ]] *
+                     MEMLOG.rep xp F (NoTransaction mbase) mscs')
 
-  CRASH             MEMLOG.would_recover_old xp mbase
+  CRASH             MEMLOG.would_recover_old xp F mbase
                     \/
-                    (exists m', MEMLOG.might_recover_cur xp mbase m' *
-                     (* Q: Even in this case, rep might not hold for (key, value) :: l because
-                           the disk might be full...How to state that here? *)
-                     [[ (rep l kv_p * F)%pred (list2mem m') ]])
-  >} put kv_p key value xp cs.
+                    (exists m', MEMLOG.would_recover_either xp F mbase m' *
+                     [[ (rep (l ++ [(key, value)]) (kv_p ^+ $1))%pred (list2mem m') ]])
+  >} put kv_p key value xp mscs.
 Proof.
+  unfold put, rep.
+  step.
+  step.
+  rewrite map_length. rewrite H8. apply wlt_lt in H4. assumption.
+  step.
+  rewrite map_length. rewrite H8. apply wlt_lt in H4. assumption.
+  step.
+  step.
+  step.
+
+  apply pimpl_or_r. left. cancel.
+  instantiate (a := upd l kv_p (key, value)).
+  repeat rewrite map_upd.
+  cancel.
+  rewrite app_length. rewrite H9. rewrite wplus_alt. unfold wplusN, wordBinN.
+  erewrite wordToNat_natToWord_bound with (bound:=maxlen). simpl. omega. simpl. apply wlt_lt in H4. omega.
+
+  rewrite length_upd. auto.
+  unfold upd. rewrite <- H9.
+
+  admit.
+
+  step.
+  step.
+  step.
+
+  unfold MEMLOG.log_intact.
+  cancel.
+(*  apply pimpl_or_r. right. cancel. *)
+  admit.
+
+  unfold MEMLOG.would_recover_old. cancel.
+  unfold MEMLOG.would_recover_old. cancel.
+  unfold MEMLOG.would_recover_old. cancel.
+  unfold MEMLOG.would_recover_old. cancel.
+
+
+  cancel.
+
+
 Admitted.
